\begin{dmath*}
{n_{ss}} = 1-{{u_{ss}}}
\end{dmath*}
\begin{dmath*}
{m_{ss}} = {{\vartheta}}\, {{n_{ss}}}
\end{dmath*}
\begin{dmath*}
{v_{ss}} = \frac{{{m_{ss}}}}{{{q_{ss}}}}
\end{dmath*}
\begin{dmath*}
{s_{ss}} = \frac{{{m_{ss}}}}{{{u_{ss}}}}
\end{dmath*}
\begin{dmath*}
{\sigma_{m}} = {{m_{ss}}}\, \left({{u_{ss}}}^{{{\xi}}}\, {{v_{ss}}}^{1-{{\xi}}}\right)^{\left(-1\right)}
\end{dmath*}
\begin{dmath*}
{\theta_{ss}} = \frac{{{v_{ss}}}}{{{u_{ss}}}}
\end{dmath*}
\begin{dmath*}
{mc_{ss}} = \frac{{{\epsilon}}-1}{{{\epsilon}}}
\end{dmath*}
\begin{dmath*}
{xL_{ss}} = {{mc_{ss}}}
\end{dmath*}
\begin{dmath*}
{R_{ss}} = \frac{1}{{{\beta}}}
\end{dmath*}
\begin{dmath*}
{n_{ss}} = \frac{{{y_{ss}}}}{{{n_{ss}}}\, {{h_{ss}}}^{{{\alpha}}}}
\end{dmath*}
\begin{dmath*}
{w_{ss}} = {{\alpha}}\, {{xL_{ss}}}\, {{n_{ss}}}\, {{h_{ss}}}^{{{\alpha}}-1}
\end{dmath*}
\begin{dmath*}
{\Phi} = \frac{{{y_{ss}}}\, {{\phi_{ss}}}}{{{n_{ss}}}}
\end{dmath*}
\begin{dmath*}
{\Psi^L_{ss}} = {{h_{ss}}}^{{{\alpha}}}\, {{xL_{ss}}}\, {{n_{ss}}}-{{h_{ss}}}\, {{w_{ss}}}-{{\Phi}}
\end{dmath*}
\begin{dmath*}
{\Psi^C_{ss}} = {{y_{ss}}}\, \left(1-{{mc_{ss}}}\right)
\end{dmath*}
\begin{dmath*}
{J_{ss}} = \frac{1}{1-{{\beta}}\, \left(1-{{\vartheta}}\right)}\, {{\Psi^L_{ss}}}
\end{dmath*}
\begin{dmath*}
{\delta^F_{ss}} = {{h_{ss}}}\, {{w_{ss}}}\, \frac{1}{1-{{\beta}}\, \left(1-{{\vartheta}}\right)\, {{\gamma}}}
\end{dmath*}
\begin{dmath*}
b = {{h_{ss}}}\, {{w_{ss}}}\, {{b_{ss}}}
\end{dmath*}
\begin{dmath*}
{mrs_{ss}} = \frac{{{w_{ss}}}\, {{h_{ss}}}\, \frac{{{\alpha}}\, \frac{{{J_{ss}}}\, {{\eta}}}{1-{{\beta}}\, \left(1-{{\vartheta}}\right)\, {{\gamma}}}}{{{\alpha}}-1}-\frac{\left(1-{{\eta}}\right)\, {{\delta^F_{ss}}}}{1-{{\beta}}\, \left(1-{{\vartheta}}-{{s_{ss}}}\right)}\, \left({{h_{ss}}}\, {{w_{ss}}}-{b}\right)}{\frac{\left(-\left(\frac{{{\eta}}\, {{h_{ss}}}\, {{J_{ss}}}}{1-{{\beta}}\, \left(1-{{\vartheta}}\right)\, {{\gamma}}}\right)\right)}{1-{{\alpha}}}-\frac{\frac{{{h_{ss}}}\, \left(1-{{\eta}}\right)\, {{\delta^F_{ss}}}}{1-{{\beta}}\, \left(1-{{\vartheta}}-{{s_{ss}}}\right)}}{1+{{\varphi}}}}
\end{dmath*}
\begin{dmath*}
{\delta^W_{ss}} = \frac{{{h_{ss}}}\, \frac{1}{1-{{\beta}}\, \left(1-{{\vartheta}}\right)\, {{\gamma}}}}{1-{{\alpha}}}\, \left({{w_{ss}}}\, \left(-{{\alpha}}\right)+{{mrs_{ss}}}\right)
\end{dmath*}
\begin{dmath*}
{\Delta_{ss}} = \frac{1}{1-{{\beta}}\, \left(1-{{\vartheta}}-{{s_{ss}}}\right)}\, \left({{h_{ss}}}\, {{w_{ss}}}-\frac{{{h_{ss}}}\, {{mrs_{ss}}}}{1+{{\varphi}}}-{b}\right)
\end{dmath*}
\begin{dmath*}
{\kappa} = {{J_{ss}}}\, {{q_{ss}}}\, {{\beta}}
\end{dmath*}
\begin{dmath*}
{c_{ss}} = {{y_{ss}}}-{{v_{ss}}}\, {{\kappa}}-{{n_{ss}}}\, {{\Phi}}-{{g_{ss}}}
\end{dmath*}
\begin{dmath*}
{\lambda_{ss}} = \left({{c_{ss}}}\, \left(1-{{\varrho}}\right)\right)^{\left(-{{\sigma}}\right)}
\end{dmath*}
\begin{dmath*}
{\kappa_L} = \frac{{{mrs_{ss}}}\, {{\lambda_{ss}}}}{{{h_{ss}}}^{{{\varphi}}}}
\end{dmath*}
\begin{dmath*}
{A_{fac}} = \frac{{{h_{ss}}}\, {{w_{ss}}}\, \frac{1-{{\alpha}}}{{{\alpha}}}}{{{\Psi^L_{ss}}}}
\end{dmath*}
% Equation 1
\begin{dmath}
{{R}}_{t}=\left(1-{{\gamma_R}}\right)\, {{\gamma_{\pi}}}\, {{\pi}}_{t-1}+\left(1-{{\gamma_R}}\right)\, {{\gamma_y}}\, {{y}}_{t}+{{\gamma_R}}\, {{R}}_{t-1}+{{e_m}}_{t}
\end{dmath}
% Equation 2
\begin{dmath}
{{\lambda}}_{t}={{R}}_{t}+{{\lambda}}_{t+1}+{{e_b}}_{t}-{{\pi}}_{t+1}
\end{dmath}
% Equation 3
\begin{dmath}
{{\lambda}}_{t}=\frac{\left(-{{\sigma}}\right)}{1-{{\varrho}}}\, \left({{c}}_{t}-{{\varrho}}\, {{c}}_{t-1}\right)
\end{dmath}
% Equation 4
\begin{dmath}
{{\pi}}_{t}={{\pi}}_{t-1}\, \frac{{{\zeta_p}}}{1+{{\beta}}\, {{\zeta_p}}}+{{\pi}}_{t+1}\, \frac{{{\beta}}}{1+{{\beta}}\, {{\zeta_p}}}+\frac{\frac{1}{1+{{\beta}}\, {{\zeta_p}}}\, \left(1-{{\omega}}\right)\, \left(1-{{\beta}}\, {{\omega}}\right)}{{{\omega}}}\, {{mc}}_{t}
\end{dmath}
% Equation 5
\begin{dmath}
{{mc}}_{t}={{xL}}_{t}
\end{dmath}
% Equation 6
\begin{dmath}
{{m}}_{t}={{\xi}}\, {{u}}_{t}+\left(1-{{\xi}}\right)\, {{v}}_{t}
\end{dmath}
% Equation 7
\begin{dmath}
{{n}}_{t}=\left(1-{{\vartheta}}\right)\, {{n}}_{t-1}+\frac{{{m_{ss}}}}{{{n_{ss}}}}\, {{m}}_{t-1}
\end{dmath}
% Equation 8
\begin{dmath}
{{n}}_{t}={{u}}_{t}\, \frac{\left(-{{u_{ss}}}\right)}{1-{{u_{ss}}}}
\end{dmath}
% Equation 9
\begin{dmath}
{{q}}_{t}={{m}}_{t}-{{v}}_{t}
\end{dmath}
% Equation 10
\begin{dmath}
{{s}}_{t}={{m}}_{t}-{{u}}_{t}
\end{dmath}
% Equation 11
\begin{dmath}
{{J^*}}_{t}+{{\delta_W}}_{t}={{\Delta^*}}_{t}+{{\delta_F}}_{t}
\end{dmath}
% Equation 12
\begin{dmath}
{{w}}_{t}={{xL}}_{t}+{{z}}_{t}+\left({{\alpha}}-1\right)\, {{h}}_{t}
\end{dmath}
% Equation 13
\begin{dmath}
{{w}}_{t}={{\gamma}}\, \left({{w}}_{t-1}-{{\pi}}_{t}+{{\pi}}_{t-1}\, {{\zeta_w}}\right)+\left(1-{{\gamma}}\right)\, {{w^*}}_{t}
\end{dmath}
% Equation 14
\begin{dmath}
{{\delta_F}}_{t}=\left(1-{{\beta}}\, \left(1-{{\vartheta}}\right)\, {{\gamma}}\right)\, \left({{w^*}}_{t}\, \frac{\left(-{{\alpha}}\right)}{1-{{\alpha}}}+\left({{xL}}_{t}+{{z}}_{t}\right)\, \frac{1}{1-{{\alpha}}}\right)+{{\beta}}\, \left(1-{{\vartheta}}\right)\, {{\gamma}}\, \left({{\lambda}}_{t+1}+\frac{\left(-{{\alpha}}\right)}{1-{{\alpha}}}\, \left({{w^*}}_{t}+{{\pi}}_{t}\, {{\zeta_w}}-{{w^*}}_{t+1}-{{\pi}}_{t+1}\right)+{{\delta_F}}_{t+1}-{{\lambda}}_{t}\right)
\end{dmath}
% Equation 15
\begin{dmath}
{{\delta_W}}_{t}\, {{\delta^W_{ss}}}=\left({{w^*}}_{t}\, \frac{\left(-{{\alpha}}\right)}{1-{{\alpha}}}+\left({{xL}}_{t}+{{z}}_{t}\right)\, \frac{1}{1-{{\alpha}}}\right)\, {{h_{ss}}}\, {{w_{ss}}}\, \frac{\left(-{{\alpha}}\right)}{1-{{\alpha}}}+{{h_{ss}}}\, {{mrs_{ss}}}\, \frac{1}{1-{{\alpha}}}\, \left({{w^*}}_{t}\, \frac{\left(-\left(1+{{\varphi}}\right)\right)}{1-{{\alpha}}}-{{\lambda}}_{t}+\left({{xL}}_{t}+{{z}}_{t}\right)\, \frac{1+{{\varphi}}}{1-{{\alpha}}}\right)+\left({{w^*}}_{t}+{{\pi}}_{t}\, {{\zeta_w}}-{{w^*}}_{t+1}-{{\pi}}_{t+1}\right)\, \frac{{{\beta}}\, \left(1-{{\vartheta}}\right)\, {{\gamma}}}{1-{{\beta}}\, \left(1-{{\vartheta}}\right)\, {{\gamma}}}\, \left({{h_{ss}}}\, {{w_{ss}}}\, \left(\frac{{{\alpha}}}{1-{{\alpha}}}\right)^{2}-{{h_{ss}}}\, {{mrs_{ss}}}\, \frac{1+{{\varphi}}}{\left(1-{{\alpha}}\right)^{2}}\right)+{{\beta}}\, \left(1-{{\vartheta}}\right)\, {{\gamma}}\, {{\delta^W_{ss}}}\, \left({{\lambda}}_{t+1}-{{\lambda}}_{t}+{{\delta_W}}_{t+1}\right)
\end{dmath}
% Equation 16
\begin{dmath}
{{J_{ss}}}\, {{J^*}}_{t}=\frac{{{h_{ss}}}\, {{w_{ss}}}}{{{\alpha}}}\, \left({{z}}_{t}+{{xL}}_{t}+\left(-{{\alpha}}\right)\, {{w^*}}_{t}\right)+{{h_{ss}}}\, {{w_{ss}}}\, \frac{{{\beta}}\, \left(1-{{\vartheta}}\right)\, {{\gamma}}}{1-{{\beta}}\, \left(1-{{\vartheta}}\right)\, {{\gamma}}}\, \left({{\pi}}_{t+1}+{{w^*}}_{t+1}-{{w^*}}_{t}-{{\pi}}_{t}\, {{\zeta_w}}\right)+{{\beta}}\, \left(1-{{\vartheta}}\right)\, {{J_{ss}}}\, \left({{\lambda}}_{t+1}-{{\lambda}}_{t}+{{J^*}}_{t+1}\right)
\end{dmath}
% Equation 17
\begin{dmath}
{{\Delta^*}}_{t}\, {{\Delta_{ss}}}=\left({{z}}_{t}+{{xL}}_{t}+\left(-{{\alpha}}\right)\, {{w^*}}_{t}\right)\, \frac{{{h_{ss}}}\, {{w_{ss}}}}{1-{{\alpha}}}-\frac{{{h_{ss}}}\, {{mrs_{ss}}}}{1+{{\varphi}}}\, \left(\frac{1+{{\varphi}}}{1-{{\alpha}}}\, \left({{z}}_{t}+{{xL}}_{t}-{{w^*}}_{t}\right)-{{\lambda}}_{t}\right)+\left({{\pi}}_{t+1}+{{w^*}}_{t+1}-{{w^*}}_{t}-{{\pi}}_{t}\, {{\zeta_w}}\right)\, \frac{{{\beta}}\, \left(1-{{\vartheta}}\right)\, {{\gamma}}}{1-{{\beta}}\, \left(1-{{\vartheta}}\right)\, {{\gamma}}}\, \left(\frac{{{\alpha}}\, {{h_{ss}}}\, {{w_{ss}}}}{1-{{\alpha}}}-{{h_{ss}}}\, {{mrs_{ss}}}\, \frac{1}{1-{{\alpha}}}\right)-\left(\frac{{{\alpha}}\, {{h_{ss}}}\, {{w_{ss}}}}{1-{{\alpha}}}-{{h_{ss}}}\, {{mrs_{ss}}}\, \frac{1}{1-{{\alpha}}}\right)\, \frac{{{s_{ss}}}\, {{\beta}}\, {{\gamma}}}{1-{{\beta}}\, \left(1-{{\vartheta}}\right)\, {{\gamma}}}\, \left({{\pi}}_{t+1}+{{w^*}}_{t+1}-{{w}}_{t}-{{\pi}}_{t}\, {{\zeta_w}}\right)+{{\beta}}\, \left(1-{{\vartheta}}-{{s_{ss}}}\right)\, {{\Delta_{ss}}}\, \left({{\lambda}}_{t+1}-{{\lambda}}_{t}+{{\Delta^*}}_{t+1}\right)-{{s}}_{t}\, {{s_{ss}}}\, {{\beta}}\, {{\Delta_{ss}}}
\end{dmath}
% Equation 18
\begin{dmath}
\frac{{{\kappa}}}{{{q_{ss}}}}\, \left(-{{q}}_{t}\right)={{h_{ss}}}\, {{w_{ss}}}\, \frac{{{\beta}}\, {{\gamma}}}{1-{{\beta}}\, \left(1-{{\vartheta}}\right)\, {{\gamma}}}\, \left({{\pi}}_{t+1}+{{w^*}}_{t+1}-{{w}}_{t}-{{\pi}}_{t}\, {{\zeta_w}}\right)+\left({{\lambda}}_{t+1}-{{\lambda}}_{t}+{{J^*}}_{t+1}\right)\, {{\beta}}\, {{J_{ss}}}
\end{dmath}
% Equation 19
\begin{dmath}
{{y_{ss}}}\, {{y}}_{t}={{c_{ss}}}\, {{c}}_{t}+{{g_{ss}}}\, {{g}}_{t}+{{v_{ss}}}\, {{\kappa}}\, {{v}}_{t}+{{n_{ss}}}\, {{\Phi}}\, {{n}}_{t}
\end{dmath}
% Equation 20
\begin{dmath}
{{y}}_{t}={{n}}_{t}+{{z}}_{t}+{{\alpha}}\, {{h}}_{t}
\end{dmath}
% Equation 21
\begin{dmath}
{{\pi_w}}_{t}={{\pi}}_{t}+{{w}}_{t}-{{w}}_{t-1}
\end{dmath}
% Equation 22
\begin{dmath}
{{\Psi^L}}_{t}={{A_{fac}}}\, \left({{w}}_{t}+{{h}}_{t}\right)
\end{dmath}
% Equation 23
\begin{dmath}
{{e_b}}_{t}={{\rho_{eb}}}\, {{e_b}}_{t-1}+{{\sigma_{eb}}}\, {{\varepsilon_{b}}}_{t}
\end{dmath}
% Equation 24
\begin{dmath}
{{g}}_{t}={{\rho_{g}}}\, {{g}}_{t-1}+{{\varepsilon_{g}}}_{t}
\end{dmath}
% Equation 25
\begin{dmath}
{{e_m}}_{t}={{\rho_{m}}}\, {{e_m}}_{t-1}+{{\sigma_{m}}}\, {{\varepsilon_{r}}}_{t}
\end{dmath}
% Equation 26
\begin{dmath}
{{z}}_{t}={{\rho_{z}}}\, {{z}}_{t-1}+{{\sigma_{z}}}\, {{\varepsilon_{z}}}_{t}
\end{dmath}
% Equation 27
\begin{dmath}
{y\_level}_{t}={{y_{ss}}}\, \left(1+{{y}}_{t}\right)
\end{dmath}
% Equation 28
\begin{dmath}
{c\_level}_{t}={{c_{ss}}}\, \left(1+{{c}}_{t}\right)
\end{dmath}
% Equation 29
\begin{dmath}
{wh\_level}_{t}={{h_{ss}}}\, {{w_{ss}}}\, \left({{h}}_{t}+1+{{w}}_{t}\right)
\end{dmath}
% Equation 30
\begin{dmath}
{u\_level}_{t}={{u_{ss}}}\, \left(1+{{u}}_{t}\right)
\end{dmath}
% Equation 31
\begin{dmath}
{v\_share\_level}_{t}={{v_{ss}}}\, \left(1+{{v}}_{t}\right)
\end{dmath}
% Equation 32
\begin{dmath}
{s\_prob\_level}_{t}={{s_{ss}}}\, \left(1+{{s}}_{t}\right)
\end{dmath}
% Equation 33
\begin{dmath}
{q\_prob\_level}_{t}={{q_{ss}}}\, \left(1+{{q}}_{t}\right)
\end{dmath}
% Equation 34
\begin{dmath}
{b\_wh\_ss}_{t}=\frac{{b}}{{{h_{ss}}}\, {{w_{ss}}}}
\end{dmath}
% Equation 35
\begin{dmath}
{kv\_y\_share\_pct\_level}_{t}=\frac{{{v_{ss}}}\, {{\kappa}}\, 100}{{{y_{ss}}}}
\end{dmath}
% Equation 36
\begin{dmath}
{F\_revenue\_share\_level}_{t}=\frac{{{\Phi}}}{{{h_{ss}}}^{{{\alpha}}}\, {{xL_{ss}}}\, {{n_{ss}}}}
\end{dmath}
% Equation 37
\begin{dmath}
{CC\_y\_share\_level}_{t}=\frac{{{\Psi^C_{ss}}}}{{{y_{ss}}}}
\end{dmath}
% Equation 38
\begin{dmath}
{CLn\_y\_share\_level}_{t}=\frac{{{n_{ss}}}\, {{\Psi^L_{ss}}}}{{{y_{ss}}}}
\end{dmath}
% Equation 39
\begin{dmath}
{J\_value\_level}_{t}={{J_{ss}}}
\end{dmath}
% Equation 40
\begin{dmath}
{D\_surplus\_level}_{t}={{\Delta_{ss}}}\, \left(1+{{\Delta^*}}_{t}\right)
\end{dmath}
