\begin{dmath*}
{\ lambda_{h}} = \frac{\left(1-{{\ beta}}\, {{\ theta_{H}}}\right)\, \left(1-{{\ theta_{H}}}\right)}{{{\ theta_{H}}}}
\end{dmath*}
\begin{dmath*}
{\ lambda_{f}} = \frac{\left(1-{{\ beta}}\, {{\ theta_{F}}}\right)\, \left(1-{{\ theta_{F}}}\right)}{{{\ theta_{F}}}}
\end{dmath*}
% Equation 1
\begin{dmath}
{{c}}_{t}-{{h}}\, {{c}}_{t-1}={{y ^ *}}_{t}-{{h}}\, {{y ^ *}}_{t-1}+\frac{1}{{{\ sigma}}}\, \left(1-{{h}}\right)\, {{q}}_{t}
\end{dmath}
% Equation 2
\begin{dmath}
{{\ pi_H}}_{t}={{\ beta}}\, \left({{\ pi_H}}_{t+1}-{{\ pi_H}}_{t}\, {{\ delta_{H}}}\right)+{{\ delta_{H}}}\, {{\ pi_H}}_{t-1}+\frac{\left(1-{{\ beta}}\, {{\ theta_{H}}}\right)\, \left(1-{{\ theta_{H}}}\right)}{{{\ theta_{H}}}}\, \left({{\ varphi}}\, {{y}}_{t}-\left(1+{{\ varphi}}\right)\, {{\ varepsilon_{a}}}_{t}+{{\ alpha}}\, {{s}}_{t}+\left({{c}}_{t}-{{h}}\, {{c}}_{t-1}\right)\, \frac{{{\ sigma}}}{1-{{h}}}\right)
\end{dmath}
% Equation 3
\begin{dmath}
{{\ pi_F}}_{t}={{\ beta}}\, \left({{\ pi_F}}_{t+1}-{{\ pi_F}}_{t}\, {{\ delta_{F}}}\right)+{{\ delta_{F}}}\, {{\ pi_F}}_{t-1}+\frac{\left(1-{{\ beta}}\, {{\ theta_{F}}}\right)\, \left(1-{{\ theta_{F}}}\right)}{{{\ theta_{F}}}}\, \left({{q}}_{t}-{{s}}_{t}\, \left(1-{{\ alpha}}\right)\right)
\end{dmath}
% Equation 4
\begin{dmath}
{{q}}_{t+1}-{{q}}_{t}={{r}}_{t}-{{\ pi}}_{t+1}-\left({{r ^ *}}_{t}-{{\ pi ^ *}}_{t+1}\right)+{{\ varepsilon_{q}}}_{t}
\end{dmath}
% Equation 5
\begin{dmath}
{{s}}_{t}-{{s}}_{t-1}={{\ pi_F}}_{t}-{{\ pi_H}}_{t}+{{\ varepsilon_{s}}}_{t}
\end{dmath}
% Equation 6
\begin{dmath}
{{y}}_{t}={{c}}_{t}\, \left(1-{{\ alpha}}\right)+{{q}}_{t}\, {{\ alpha}}\, {{\ eta}}+{{s}}_{t}\, {{\ alpha}}\, {{\ eta}}+{{y ^ *}}_{t}\, {{\ alpha}}
\end{dmath}
% Equation 7
\begin{dmath}
{{\ pi}}_{t}={{\ pi_H}}_{t}\, \left(1-{{\ alpha}}\right)+{{\ alpha}}\, {{\ pi_F}}_{t}
\end{dmath}
% Equation 8
\begin{dmath}
{{r}}_{t}={{\ psi_{r}}}\, {{r}}_{t-1}+\left(1-{{\ psi_{r}}}\right)\, \left({{\ pi}}_{t}\, {{\ psi_{\ pi}}}+{{y}}_{t}\, {{\ psi_{y}}}+{{\ psi_{de}}}\, \left({{e}}_{t}-{{e}}_{t-1}\right)\right)+{{\ varepsilon_{r}}}_{t}
\end{dmath}
% Equation 9
\begin{dmath}
{{\ Delta e}}_{t}={{e}}_{t}-{{e}}_{t-1}
\end{dmath}
% Equation 10
\begin{dmath}
{{q}}_{t}-{{q}}_{t-1}={{\ Delta e}}_{t}+{{\ pi ^ *}}_{t}-{{\ pi}}_{t}
\end{dmath}
% Equation 11
\begin{dmath}
{{\ varepsilon_{r}}}_{t}={{\ rho_{r}}}\, {{\ varepsilon_{r}}}_{t-1}+{{e_{r}}}_{t}
\end{dmath}
% Equation 12
\begin{dmath}
{{\ varepsilon_{s}}}_{t}={{\ rho_{s}}}\, {{\ varepsilon_{s}}}_{t-1}+{{e_{s}}}_{t}
\end{dmath}
% Equation 13
\begin{dmath}
{{\ varepsilon_{q}}}_{t}={{\ rho_{q}}}\, {{\ varepsilon_{q}}}_{t-1}+{{e_{q}}}_{t}
\end{dmath}
% Equation 14
\begin{dmath}
{{\ varepsilon_{a}}}_{t}={{\ rho_{a}}}\, {{\ varepsilon_{a}}}_{t-1}+{{e_{a}}}_{t}
\end{dmath}
% Equation 15
\begin{dmath}
{{\ pi ^ *}}_{t}={{a_1}}\, {{\ pi ^ *}}_{t-1}+{{e_{\ pi ^ *}}}_{t}
\end{dmath}
% Equation 16
\begin{dmath}
{{y ^ *}}_{t}={{y ^ *}}_{t-1}\, {{b_1}}+{{e_{y ^ *}}}_{t}
\end{dmath}
% Equation 17
\begin{dmath}
{{r ^ *}}_{t}={{c_1}}\, {{r ^ *}}_{t-1}+{{e_{r ^ *}}}_{t}
\end{dmath}
% Equation 18
\begin{dmath}
{y\_obs}_{t}={{y}}_{t}
\end{dmath}
% Equation 19
\begin{dmath}
{yst\_obs}_{t}={{y ^ *}}_{t}
\end{dmath}
% Equation 20
\begin{dmath}
{r\_obs}_{t}={{r}}_{t}\, 4
\end{dmath}
% Equation 21
\begin{dmath}
{pi\_obs}_{t}={{\ pi}}_{t}\, 4
\end{dmath}
% Equation 22
\begin{dmath}
{q\_obs}_{t}={{q}}_{t}
\end{dmath}
% Equation 23
\begin{dmath}
{s\_obs}_{t}={{s}}_{t}
\end{dmath}
% Equation 24
\begin{dmath}
{pif\_obs}_{t}={{\ pi ^ *}}_{t}\, 4
\end{dmath}
% Equation 25
\begin{dmath}
{rst\_obs}_{t}={{r ^ *}}_{t}\, 4
\end{dmath}
