\begin{dmath*}
cpie = 1+\frac{{{\bar \pi}}}{100}
\end{dmath*}
\begin{dmath*}
cgamma = 1+\frac{{{\bar \gamma}}}{100}
\end{dmath*}
\begin{dmath*}
cbeta = \frac{1}{1+\frac{{{100(\beta^{-1}-1)}}}{100}}
\end{dmath*}
\begin{dmath*}
clandap = {{\Phi}}
\end{dmath*}
\begin{dmath*}
cbetabar = {cbeta}\, {cgamma}^{\left(-{{\sigma_c}}\right)}
\end{dmath*}
\begin{dmath*}
cr = \frac{{cpie}}{{cbeta}\, {cgamma}^{\left(-{{\sigma_c}}\right)}}
\end{dmath*}
\begin{dmath*}
crk = {cbeta}^{\left(-1\right)}\, {cgamma}^{{{\sigma_c}}}-\left(1-{{\delta}}\right)
\end{dmath*}
\begin{dmath*}
cw = \left(\frac{{{\alpha}}^{{{\alpha}}}\, \left(1-{{\alpha}}\right)^{1-{{\alpha}}}}{{clandap}\, {crk}^{{{\alpha}}}}\right)^{\frac{1}{1-{{\alpha}}}}
\end{dmath*}
\begin{dmath*}
cikbar = 1-\frac{1-{{\delta}}}{{cgamma}}
\end{dmath*}
\begin{dmath*}
cik = {cgamma}\, \left(1-\frac{1-{{\delta}}}{{cgamma}}\right)
\end{dmath*}
\begin{dmath*}
clk = \frac{1-{{\alpha}}}{{{\alpha}}}\, \frac{{crk}}{{cw}}
\end{dmath*}
\begin{dmath*}
cky = {{\Phi}}\, {clk}^{{{\alpha}}-1}
\end{dmath*}
\begin{dmath*}
ciy = {cik}\, {cky}
\end{dmath*}
\begin{dmath*}
ccy = 1-{{\frac{\bar g}{\bar y}}}-{cik}\, {cky}
\end{dmath*}
\begin{dmath*}
crkky = {crk}\, {cky}
\end{dmath*}
\begin{dmath*}
cwhlc = \frac{{cky}\, {crk}\, \frac{\left(1-{{\alpha}}\right)\, \frac{1}{{{\phi_w}}}}{{{\alpha}}}}{{ccy}}
\end{dmath*}
\begin{dmath*}
cwly = 1-{crk}\, {cky}
\end{dmath*}
\begin{dmath*}
conster = 100\, \left({cr}-1\right)
\end{dmath*}
\begin{dmath*}
c1 = \frac{\frac{{{\lambda}}}{{cgamma}}}{1+\frac{{{\lambda}}}{{cgamma}}}
\end{dmath*}
\begin{dmath*}
c2 = \frac{\left({{\sigma_c}}-1\right)\, {cwhlc}}{{{\sigma_c}}\, \left(1+\frac{{{\lambda}}}{{cgamma}}\right)}
\end{dmath*}
\begin{dmath*}
c3 = \frac{1-\frac{{{\lambda}}}{{cgamma}}}{{{\sigma_c}}\, \left(1+\frac{{{\lambda}}}{{cgamma}}\right)}
\end{dmath*}
\begin{dmath*}
i1 = \frac{1}{1+{cgamma}\, {cbetabar}}
\end{dmath*}
\begin{dmath*}
i2 = \frac{1}{1+{cgamma}\, {cbetabar}}\, \frac{1}{{cgamma}^{2}\, {{\varphi}}}
\end{dmath*}
\begin{dmath*}
q1 = \frac{1-{{\delta}}}{1-{{\delta}}+{crk}}
\end{dmath*}
\begin{dmath*}
q2 = \frac{1}{\frac{1-\frac{{{\lambda}}}{{cgamma}}}{{{\sigma_c}}\, \left(1+\frac{{{\lambda}}}{{cgamma}}\right)}}
\end{dmath*}
\begin{dmath*}
k1 = 1-{cikbar}
\end{dmath*}
\begin{dmath*}
k2 = {{\varphi}}\, {cgamma}^{2}\, {cikbar}
\end{dmath*}
\begin{dmath*}
pi1 = {{\iota_p}}\, \frac{1}{1+{cgamma}\, {cbetabar}\, {{\iota_p}}}
\end{dmath*}
\begin{dmath*}
pi2 = {cgamma}\, {cbetabar}\, \frac{1}{1+{cgamma}\, {cbetabar}\, {{\iota_p}}}
\end{dmath*}
\begin{dmath*}
pi3 = \frac{\frac{1}{1+{cgamma}\, {cbetabar}\, {{\iota_p}}}\, \frac{\left(1-{{\xi_p}}\right)\, \left(1-{cgamma}\, {cbetabar}\, {{\xi_p}}\right)}{{{\xi_p}}}}{1+\left({{\Phi}}-1\right)\, {{\varepsilon_p}}}
\end{dmath*}
\begin{dmath*}
w1 = \frac{1}{1+{cgamma}\, {cbetabar}}
\end{dmath*}
\begin{dmath*}
w2 = \frac{1+{cgamma}\, {cbetabar}\, {{\iota_w}}}{1+{cgamma}\, {cbetabar}}
\end{dmath*}
\begin{dmath*}
w3 = \frac{{{\iota_w}}}{1+{cgamma}\, {cbetabar}}
\end{dmath*}
\begin{dmath*}
w4 = \frac{\left(1-{{\xi_w}}\right)\, \left(1-{cgamma}\, {cbetabar}\, {{\xi_w}}\right)}{\left(1+{cgamma}\, {cbetabar}\right)\, {{\xi_w}}}\, \frac{1}{1+\left({{\phi_w}}-1\right)\, {{\varepsilon_w}}}
\end{dmath*}
\begin{dmath*}
w5 = \frac{1}{1-\frac{{{\lambda}}}{{cgamma}}}
\end{dmath*}
\begin{dmath*}
w6 = \frac{\frac{{{\lambda}}}{{cgamma}}}{1-\frac{{{\lambda}}}{{cgamma}}}
\end{dmath*}
% Equation 1
\begin{dmath}
{{\varepsilon_a}}_{t}={{\alpha}}\, {{r^{k,flex}}}_{t}+\left(1-{{\alpha}}\right)\, {{w^{flex}}}_{t}
\end{dmath}
% Equation 2
\begin{dmath}
{{z^{flex}}}_{t}={{r^{k,flex}}}_{t}\, \frac{1}{\frac{{{\psi}}}{1-{{\psi}}}}
\end{dmath}
% Equation 3
\begin{dmath}
{{r^{k,flex}}}_{t}={{w^{flex}}}_{t}+{{l^{flex}}}_{t}-{{k^{s,flex}}}_{t}
\end{dmath}
% Equation 4
\begin{dmath}
{{k^{s,flex}}}_{t}={{z^{flex}}}_{t}+{{k^{flex}}}_{t-1}
\end{dmath}
% Equation 5
\begin{dmath}
{{i^{flex}}}_{t}={i1}\, {{i^{flex}}}_{t-1}+\left(1-{i1}\right)\, {{i^{flex}}}_{t+1}+{i2}\, {{q^{flex}}}_{t}+{{\varepsilon^i}}_{t}
\end{dmath}
% Equation 6
\begin{dmath}
{{q^{flex}}}_{t}={q1}\, {{q^{flex}}}_{t+1}+\left(1-{q1}\right)\, {{r^{k,flex}}}_{t+1}+{q2}\, {{c_2*\varepsilon_t^b}}_{t}-{{r^{flex}}}_{t}
\end{dmath}
% Equation 7
\begin{dmath}
{{c^{flex}}}_{t}={{c_2*\varepsilon_t^b}}_{t}+{c1}\, {{c^{flex}}}_{t-1}+\left(1-{c1}\right)\, {{c^{flex}}}_{t+1}+{c2}\, \left({{l^{flex}}}_{t}-{{l^{flex}}}_{t+1}\right)-{{r^{flex}}}_{t}\, {c3}
\end{dmath}
% Equation 8
\begin{dmath}
{{y^{flex}}}_{t}={ccy}\, {{c^{flex}}}_{t}+{{i^{flex}}}_{t}\, {ciy}+{{\varepsilon^g}}_{t}+{{z^{flex}}}_{t}\, {crkky}
\end{dmath}
% Equation 9
\begin{dmath}
{{y^{flex}}}_{t}={{\Phi}}\, \left({{\varepsilon_a}}_{t}+{{\alpha}}\, {{k^{s,flex}}}_{t}+\left(1-{{\alpha}}\right)\, {{l^{flex}}}_{t}\right)
\end{dmath}
% Equation 10
\begin{dmath}
{{w^{flex}}}_{t}={{l^{flex}}}_{t}\, {{\sigma_l}}+{{c^{flex}}}_{t}\, {w5}-{{c^{flex}}}_{t-1}\, {w6}
\end{dmath}
% Equation 11
\begin{dmath}
{{k^{flex}}}_{t}={{k^{flex}}}_{t-1}\, {k1}+{{i^{flex}}}_{t}\, \left(1-{k1}\right)+{{\varepsilon^i}}_{t}\, {k2}
\end{dmath}
% Equation 12
\begin{dmath}
{{\mu_p}}_{t}={{\alpha}}\, {{r^{k}}}_{t}+\left(1-{{\alpha}}\right)\, {{w}}_{t}-{{\varepsilon_a}}_{t}
\end{dmath}
% Equation 13
\begin{dmath}
{{z}}_{t}=\frac{1}{\frac{{{\psi}}}{1-{{\psi}}}}\, {{r^{k}}}_{t}
\end{dmath}
% Equation 14
\begin{dmath}
{{r^{k}}}_{t}={{w}}_{t}+{{l}}_{t}-{{k^{s}}}_{t}
\end{dmath}
% Equation 15
\begin{dmath}
{{k^{s}}}_{t}={{z}}_{t}+{{k}}_{t-1}
\end{dmath}
% Equation 16
\begin{dmath}
{{k}}_{t}={{\varepsilon^i}}_{t}\, {k2}+{k1}\, {{k}}_{t-1}+\left(1-{k1}\right)\, {{i}}_{t}
\end{dmath}
% Equation 17
\begin{dmath}
{{i}}_{t}={{\varepsilon^i}}_{t}+{i1}\, {{i}}_{t-1}+\left(1-{i1}\right)\, {{i}}_{t+1}+{i2}\, {{q}}_{t}
\end{dmath}
% Equation 18
\begin{dmath}
{{q}}_{t}={q2}\, {{c_2*\varepsilon_t^b}}_{t}+{q1}\, {{q}}_{t+1}+\left(1-{q1}\right)\, {{r^{k}}}_{t+1}-\left({{r}}_{t}-{{\pi}}_{t+1}\right)
\end{dmath}
% Equation 19
\begin{dmath}
{{c}}_{t}={{c_2*\varepsilon_t^b}}_{t}+{c1}\, {{c}}_{t-1}+\left(1-{c1}\right)\, {{c}}_{t+1}+{c2}\, \left({{l}}_{t}-{{l}}_{t+1}\right)-{c3}\, \left({{r}}_{t}-{{\pi}}_{t+1}\right)
\end{dmath}
% Equation 20
\begin{dmath}
{{y}}_{t}={{\varepsilon^g}}_{t}+{ccy}\, {{c}}_{t}+{ciy}\, {{i}}_{t}+{crkky}\, {{z}}_{t}
\end{dmath}
% Equation 21
\begin{dmath}
{{y}}_{t}={{\Phi}}\, \left({{\varepsilon_a}}_{t}+{{\alpha}}\, {{k^{s}}}_{t}+\left(1-{{\alpha}}\right)\, {{l}}_{t}\right)
\end{dmath}
% Equation 22
\begin{dmath}
{{\pi}}_{t}={pi1}\, {{\pi}}_{t-1}+{{\pi}}_{t+1}\, {pi2}+{{\mu_p}}_{t}\, {pi3}+{{\varepsilon^p}}_{t}
\end{dmath}
% Equation 23
\begin{dmath}
{{w}}_{t}={w1}\, {{w}}_{t-1}+\left(1-{w1}\right)\, \left({{\pi}}_{t+1}+{{w}}_{t+1}\right)-{{\pi}}_{t}\, {w2}+{{\pi}}_{t-1}\, {w3}-{w4}\, {{\mu_w}}_{t}+{{\varepsilon^w}}_{t}
\end{dmath}
% Equation 24
\begin{dmath}
{{\mu_w}}_{t}={{w}}_{t}-\left({{\sigma_l}}\, {{l}}_{t}+\frac{1}{1-\frac{{{\lambda}}}{{cgamma}}}\, \left({{c}}_{t}-\frac{{{\lambda}}}{{cgamma}}\, {{c}}_{t-1}\right)\right)
\end{dmath}
% Equation 25
\begin{dmath}
{{r}}_{t}={{\pi}}_{t}\, {{r_{\pi}}}\, \left(1-{{\rho}}\right)+\left(1-{{\rho}}\right)\, {{r_{y}}}\, \left({{y}}_{t}-{{y^{flex}}}_{t}\right)+{{r_{\Delta y}}}\, \left({{y}}_{t}-{{y^{flex}}}_{t}-{{y}}_{t-1}+{{y^{flex}}}_{t-1}\right)+{{\rho}}\, {{r}}_{t-1}+{{\varepsilon^r}}_{t}
\end{dmath}
% Equation 26
\begin{dmath}
{{\varepsilon_a}}_{t}={{\rho_a}}\, {{\varepsilon_a}}_{t-1}+{{\eta^a}}_{t}
\end{dmath}
% Equation 27
\begin{dmath}
{{c_2*\varepsilon_t^b}}_{t}={{\rho_b}}\, {{c_2*\varepsilon_t^b}}_{t-1}+{{\eta^b}}_{t}
\end{dmath}
% Equation 28
\begin{dmath}
{{\varepsilon^g}}_{t}={{\rho_g}}\, {{\varepsilon^g}}_{t-1}+{{\eta^g}}_{t}+{{\eta^a}}_{t}\, {{\rho_{ga}}}
\end{dmath}
% Equation 29
\begin{dmath}
{{\varepsilon^i}}_{t}={{\rho_i}}\, {{\varepsilon^i}}_{t-1}+{{\eta^i}}_{t}
\end{dmath}
% Equation 30
\begin{dmath}
{{\varepsilon^r}}_{t}={{\rho_r}}\, {{\varepsilon^r}}_{t-1}+{{\eta^m}}_{t}
\end{dmath}
% Equation 31
\begin{dmath}
{{\varepsilon^p}}_{t}={{\rho_p}}\, {{\varepsilon^p}}_{t-1}+{{\eta^{p,aux}}}_{t}-{{\mu_p}}\, {{\eta^{p,aux}}}_{t-1}
\end{dmath}
% Equation 32
\begin{dmath}
{{\eta^{p,aux}}}_{t}={{\eta^{p}}}_{t}
\end{dmath}
% Equation 33
\begin{dmath}
{{\varepsilon^w}}_{t}={{\rho_w}}\, {{\varepsilon^w}}_{t-1}+{{\eta^{w,aux}}}_{t}-{{\mu_w}}\, {{\eta^{w,aux}}}_{t-1}
\end{dmath}
% Equation 34
\begin{dmath}
{{\eta^{w,aux}}}_{t}={{\eta^{w}}}_{t}
\end{dmath}
% Equation 35
\begin{dmath}
{{dlGDP}}_{t}={{\bar \gamma}}+{{y}}_{t}-{{y}}_{t-1}
\end{dmath}
% Equation 36
\begin{dmath}
{{dlCONS}}_{t}={{\bar \gamma}}+{{c}}_{t}-{{c}}_{t-1}
\end{dmath}
% Equation 37
\begin{dmath}
{{dlINV}}_{t}={{\bar \gamma}}+{{i}}_{t}-{{i}}_{t-1}
\end{dmath}
% Equation 38
\begin{dmath}
{{dlWAG}}_{t}={{\bar \gamma}}+{{w}}_{t}-{{w}}_{t-1}
\end{dmath}
% Equation 39
\begin{dmath}
{{dlP}}_{t}={{\bar \pi}}+{{\pi}}_{t}
\end{dmath}
% Equation 40
\begin{dmath}
{{FEDFUNDS}}_{t}={{r}}_{t}+{conster}
\end{dmath}
% Equation 41
\begin{dmath}
{{lHOURS}}_{t}={{l}}_{t}+{{\bar l}}
\end{dmath}
