\begin{dmath*}
cbetabar = {{\beta}}\, \exp\left(\left(1-{{\sigma_c}}\right)\, {{\gamma}}\right)
\end{dmath*}
\begin{dmath*}
cpie = 1+\frac{{{\bar \pi}}}{100}
\end{dmath*}
\begin{dmath*}
crss = \frac{{cpie}}{{cbetabar}}
\end{dmath*}
\begin{dmath*}
clandap = {{\Phi}}
\end{dmath*}
\begin{dmath*}
c1 = \frac{{{\lambda}}\, \exp\left(\left(-{{\gamma}}\right)\right)}{1+{{\lambda}}\, \exp\left(\left(-{{\gamma}}\right)\right)}
\end{dmath*}
\begin{dmath*}
c2 = \frac{1-{{\lambda}}\, \exp\left(\left(-{{\gamma}}\right)\right)}{{{\sigma_c}}\, \left(1+{{\lambda}}\, \exp\left(\left(-{{\gamma}}\right)\right)\right)}
\end{dmath*}
\begin{dmath*}
c3 = \frac{1}{1+{{\lambda}}\, \exp\left(\left(-{{\gamma}}\right)\right)}
\end{dmath*}
\begin{dmath*}
c4 = \frac{1}{1-{{\alpha}}}\, \left({{\rho_a}}-1\right)
\end{dmath*}
\begin{dmath*}
c5 = \frac{\left({{\sigma_c}}-1\right)\, {{wl_c}}}{{{\sigma_c}}\, \left(1+{{\lambda}}\, \exp\left(\left(-{{\gamma}}\right)\right)\right)}
\end{dmath*}
\begin{dmath*}
i1 = \frac{1}{1+{cbetabar}}
\end{dmath*}
\begin{dmath*}
i2 = \frac{{cbetabar}}{1+{cbetabar}}
\end{dmath*}
\begin{dmath*}
i3 = \left(1+{cbetabar}\right)\, {{\varphi}}\, \exp\left(2\, {{\gamma}}\right)
\end{dmath*}
\begin{dmath*}
k1 = 1-\frac{{{\frac{\bar i}{\bar y}}}}{{{\bar k^*}}}
\end{dmath*}
\begin{dmath*}
k2 = \frac{{{\frac{\bar i}{\bar y}}}}{{{\bar k^*}}}
\end{dmath*}
\begin{dmath*}
k3 = \frac{\left(1+{cbetabar}\right)\, \exp\left(2\, {{\gamma}}\right)\, {{\varphi}}\, {{\frac{\bar i}{\bar y}}}}{{{\bar k^*}}}
\end{dmath*}
\begin{dmath*}
u1 = \frac{1-{{\psi}}}{{{\psi}}}
\end{dmath*}
\begin{dmath*}
pi1 = \frac{\left(1-{cbetabar}\, {{\xi_p}}\right)\, \left(1-{{\xi_p}}\right)}{{{\xi_p}}\, \left(1+\left({{\Phi}}-1\right)\, {{\varepsilon_w}}\right)}
\end{dmath*}
\begin{dmath*}
pi2 = \frac{1}{1+{cbetabar}\, {{\iota_p}}}
\end{dmath*}
\begin{dmath*}
pi3 = \frac{{{\iota_p}}}{1+{cbetabar}\, {{\iota_p}}}
\end{dmath*}
\begin{dmath*}
pi4 = \frac{{cbetabar}}{1+{cbetabar}\, {{\iota_p}}}
\end{dmath*}
\begin{dmath*}
w1 = \frac{\left(1-{cbetabar}\, {{\xi_w}}\right)\, \left(1-{{\xi_w}}\right)}{{{\xi_w}}\, \left(1+0.5\, {{\varepsilon_p}}\right)}
\end{dmath*}
\begin{dmath*}
w2 = \frac{1}{1+{cbetabar}}
\end{dmath*}
\begin{dmath*}
w3 = \frac{1+{cbetabar}\, {{\iota_w}}}{1+{cbetabar}}
\end{dmath*}
\begin{dmath*}
w4 = \frac{{cbetabar}}{1+{cbetabar}}
\end{dmath*}
\begin{dmath*}
y1 = \frac{{{\frac{\bar c}{\bar y}}}}{{{\frac{\bar {yp}}{\bar y}}}}
\end{dmath*}
\begin{dmath*}
y2 = \frac{{{\frac{\bar i}{\bar y}}}}{{{\frac{\bar {yp}}{\bar y}}}}
\end{dmath*}
\begin{dmath*}
y3 = {{\bar {rk}}}\, \frac{{{k^*}}}{{{\frac{\bar {yp}}{\bar y}}}}
\end{dmath*}
\begin{dmath*}
ff1 = \frac{{{\bar {rk}}}}{1+{{\bar {rk}}}-{{\delta}}}
\end{dmath*}
\begin{dmath*}
ff2 = \frac{1-{{\delta}}}{1+{{\bar {rk}}}-{{\delta}}}
\end{dmath*}
\begin{dmath*}
ff3 = \frac{{{\sigma_c}}\, \left(1+{{\lambda}}\, \exp\left(\left(-{{\gamma}}\right)\right)\right)}{1-{{\lambda}}\, \exp\left(\left(-{{\gamma}}\right)\right)}
\end{dmath*}
\begin{dmath*}
ff4 = \frac{{{\gamma^*}}\, {{v^*}}}{{{n_*}}}
\end{dmath*}
\begin{dmath*}
mrs1 = \frac{1}{1-{{\lambda}}\, \exp\left(\left(-{{\gamma}}\right)\right)}
\end{dmath*}
% Equation 1
\begin{dmath}
{{c}}_{t}=\left(-{c2}\right)\, \left({{r}}_{t}-{{\pi}}_{t+1}\right)+{{c_2*\varepsilon_t^b}}_{t}+{c1}\, \left({{c}}_{t-1}-{{w}}_{t}\right)+{c3}\, \left({{c}}_{t+1}+{c4}\, {{z^{til}}}_{t}\right)+{c5}\, \left({{l}}_{t}-{{l}}_{t+1}\right)
\end{dmath}
% Equation 2
\begin{dmath}
{{q}}_{t}={i3}\, \left({{i}}_{t}-{i1}\, \left({{i}}_{t-1}-{{w}}_{t}\right)-{i2}\, {{i}}_{t+1}-{{z^{til}}}_{t}\, {c4}\, {i2}-{{\varepsilon^i}}_{t}\right)
\end{dmath}
% Equation 3
\begin{dmath}
{{k}}_{t}={k1}\, \left({{k}}_{t-1}-{{w}}_{t}\right)+{{i}}_{t}\, {k2}+{{\varepsilon^i}}_{t}\, {k3}
\end{dmath}
% Equation 4
\begin{dmath}
{{k^{s}}}_{t}={{k}}_{t-1}+{{u}}_{t}-{{w}}_{t}
\end{dmath}
% Equation 5
\begin{dmath}
{{u}}_{t}={u1}\, {{r^{k}}}_{t}
\end{dmath}
% Equation 6
\begin{dmath}
{{\mu_p}}_{t}={{w}}_{t}+{{\alpha}}\, {{l}}_{t}-{{\alpha}}\, {{k^{s}}}_{t}
\end{dmath}
% Equation 7
\begin{dmath}
{{k^{s}}}_{t}={{l}}_{t}+{{w}}_{t}-{{r^{k}}}_{t}
\end{dmath}
% Equation 8
\begin{dmath}
{{y}}_{t}={{k^{s}}}_{t}\, {{\Phi}}\, {{\alpha}}+{{l}}_{t}\, {{\Phi}}\, \left(1-{{\alpha}}\right)+{{z^{til}}}_{t}\, \frac{{{\Phi}}-1}{1-{{\alpha}}}
\end{dmath}
% Equation 9
\begin{dmath}
{{y}}_{t}={{\frac{\bar g}{\bar y}}}\, {{\varepsilon^g}}_{t}+{{c}}_{t}\, {y1}+{{i}}_{t}\, {y2}+{{u}}_{t}\, {y3}-{{z^{til}}}_{t}\, {c4}\, {{\frac{\bar g}{\bar y}}}
\end{dmath}
% Equation 10
\begin{dmath}
{{\pi}}_{t}={{\mu_p}}_{t}\, {pi1}\, {pi2}+{pi3}\, {{\pi}}_{t-1}+{{\pi}}_{t+1}\, {pi4}+{{\varepsilon^p}}_{t}
\end{dmath}
% Equation 11
\begin{dmath}
{{w}}_{t}={w1}\, {w2}\, \left({{w^{h}}}_{t}-{{w}}_{t}\right)-{{\pi}}_{t}\, {w3}+{w2}\, \left({{w}}_{t-1}-{{w}}_{t}+{{\iota_w}}\, {{\pi}}_{t-1}\right)+{w4}\, \left({{\pi}}_{t+1}+{c4}\, {{z^{til}}}_{t}+{{w}}_{t+1}\right)+{{\varepsilon^w}}_{t}
\end{dmath}
% Equation 12
\begin{dmath}
{{w^{h}}}_{t}={mrs1}\, \left({{c}}_{t}-{{\lambda}}\, \exp\left(\left(-{{\gamma}}\right)\right)\, {{c}}_{t-1}+{{\lambda}}\, \exp\left(\left(-{{\gamma}}\right)\right)\, {{w}}_{t}\right)+{{l}}_{t}\, {{\sigma_l}}
\end{dmath}
% Equation 13
\begin{dmath}
{{r}}_{t}={{\rho}}\, {{r}}_{t-1}+\left(1-{{\rho}}\right)\, {{r_{\pi}}}\, \left({{\pi}}_{t}-{{\pi_*}}_{t}\right)+\left(1-{{\rho}}\right)\, {{r_{y}}}\, \left({{y}}_{t}-{{y^{flex}}}_{t}\right)+{{r_{\Delta y}}}\, \left({{y}}_{t}-{{y^{flex}}}_{t}-\left({{y}}_{t-1}-{{y^{flex}}}_{t-1}\right)\right)+{{\varepsilon^r}}_{t}
\end{dmath}
% Equation 14
\begin{dmath}
{{r^{ktil}}}_{t}={{\pi}}_{t}+{{r^{k}}}_{t}\, {ff1}+{{q}}_{t}\, {ff2}-{{q}}_{t-1}
\end{dmath}
% Equation 15
\begin{dmath}
{{r^{ktil}}}_{t+1}-{{r}}_{t}={{c_2*\varepsilon_t^b}}_{t}\, \left(-{ff3}\right)+{{\zeta_{sp}}}\, \left({{q}}_{t}+{{k}}_{t}-{{n}}_{t}\right)+{{\sigma_w}}_{t}
\end{dmath}
% Equation 16
\begin{dmath}
{{n}}_{t}={{\zeta_{nRk}}}\, \left({{r^{ktil}}}_{t}-{{\pi}}_{t}\right)-{{\zeta_{nR}}}\, \left({{r}}_{t-1}-{{\pi}}_{t}\right)+{{\zeta_{nqk}}}\, \left({{k}}_{t-1}+{{q}}_{t-1}\right)+{{\zeta_{nn}}}\, {{n}}_{t-1}-\frac{{{\zeta_{n\sigma_{w}}}}}{{{\zeta_{sp\sigma_{w}}}}}\, {{\sigma_w}}_{t-1}-{{w}}_{t}\, {ff4}
\end{dmath}
% Equation 17
\begin{dmath}
{{c^{flex}}}_{t}={{c_2*\varepsilon_t^b}}_{t}+\left(-{c2}\right)\, {{r^{flex}}}_{t}+{c1}\, \left({{c^{flex}}}_{t-1}-{{w}}_{t}\right)+{c3}\, \left({c4}\, {{z^{til}}}_{t}+{{c^{flex}}}_{t+1}\right)+{c5}\, \left({{l^{flex}}}_{t}-{{l^{flex}}}_{t+1}\right)
\end{dmath}
% Equation 18
\begin{dmath}
{{q^{flex}}}_{t}={i3}\, \left({{i^{flex}}}_{t}-{i1}\, \left({{i^{flex}}}_{t-1}-{{w}}_{t}\right)-{i2}\, {{i^{flex}}}_{t+1}-{{z^{til}}}_{t}\, {c4}\, {i2}-{{\varepsilon^i}}_{t}\right)
\end{dmath}
% Equation 19
\begin{dmath}
{{k^{flex}}}_{t}={{\varepsilon^i}}_{t}\, {k3}+{k1}\, \left({{k^{flex}}}_{t-1}-{{w}}_{t}\right)+{k2}\, {{i^{flex}}}_{t}
\end{dmath}
% Equation 20
\begin{dmath}
{{k^{s,flex}}}_{t}={{k^{flex}}}_{t-1}+{{z^{flex}}}_{t}-{{w}}_{t}
\end{dmath}
% Equation 21
\begin{dmath}
{{z^{flex}}}_{t}={u1}\, {{r^{k,flex}}}_{t}
\end{dmath}
% Equation 22
\begin{dmath}
{{w^{flex}}}_{t}={{l^{flex}}}_{t}\, \left(-{{\alpha}}\right)+{{\alpha}}\, {{k^{s,flex}}}_{t}
\end{dmath}
% Equation 23
\begin{dmath}
{{k^{s,flex}}}_{t}={{l^{flex}}}_{t}+{{w^{flex}}}_{t}-{{r^{k,flex}}}_{t}
\end{dmath}
% Equation 24
\begin{dmath}
{{y^{flex}}}_{t}={{z^{til}}}_{t}\, \frac{{{\Phi}}-1}{1-{{\alpha}}}+{{\Phi}}\, {{\alpha}}\, {{k^{s,flex}}}_{t}+{{\Phi}}\, \left(1-{{\alpha}}\right)\, {{l^{flex}}}_{t}
\end{dmath}
% Equation 25
\begin{dmath}
{{y^{flex}}}_{t}={{\frac{\bar g}{\bar y}}}\, {{\varepsilon^g}}_{t}+{y1}\, {{c^{flex}}}_{t}+{y2}\, {{i^{flex}}}_{t}+{y3}\, {{z^{flex}}}_{t}-{{z^{til}}}_{t}\, {c4}\, {{\frac{\bar g}{\bar y}}}
\end{dmath}
% Equation 26
\begin{dmath}
{{w^{flex}}}_{t}={mrs1}\, \left({{\lambda}}\, \exp\left(\left(-{{\gamma}}\right)\right)\, {{w}}_{t}+{{c^{flex}}}_{t}-{{\lambda}}\, \exp\left(\left(-{{\gamma}}\right)\right)\, {{c^{flex}}}_{t-1}\right)+{{\sigma_l}}\, {{l^{flex}}}_{t}
\end{dmath}
% Equation 27
\begin{dmath}
{{q^{flex}}}_{t}={ff1}\, {{r^{k,flex}}}_{t+1}+{ff2}\, {{q^{flex}}}_{t+1}-{{r^{flex}}}_{t}+{{c_2*\varepsilon_t^b}}_{t}\, {ff3}
\end{dmath}
% Equation 28
\begin{dmath}
{{OG}}_{t}={{y}}_{t}-{{y^{flex}}}_{t}
\end{dmath}
% Equation 29
\begin{dmath}
{{w}}_{t}={c4}\, {{z^{til}}}_{t-1}+\frac{1}{1-{{\alpha}}}\, {{\eta^a}}_{t}+{{z_p}}_{t}
\end{dmath}
% Equation 30
\begin{dmath}
{{z^{til}}}_{t}={{\eta^a}}_{t}+{{\rho_a}}\, {{z^{til}}}_{t-1}
\end{dmath}
% Equation 31
\begin{dmath}
{{\varepsilon^g}}_{t}={{\rho_g}}\, {{\varepsilon^g}}_{t-1}+{{\eta^g}}_{t}+{{\eta^a}}_{t}\, {{\rho_{ga}}}
\end{dmath}
% Equation 32
\begin{dmath}
{{c_2*\varepsilon_t^b}}_{t}={{\rho_b}}\, {{c_2*\varepsilon_t^b}}_{t-1}+{{\eta^b}}_{t}
\end{dmath}
% Equation 33
\begin{dmath}
{{\varepsilon^i}}_{t}={{\rho_i}}\, {{\varepsilon^i}}_{t-1}+{{\eta^i}}_{t}
\end{dmath}
% Equation 34
\begin{dmath}
{{\varepsilon^p}}_{t}={{\rho_p}}\, {{\varepsilon^p}}_{t-1}+{{\eta^{p}}}_{t}-{{\mu_p}}\, {{\sigma_{map}}}\, {{\eta^{p}}}_{t-1}
\end{dmath}
% Equation 35
\begin{dmath}
{{\varepsilon^w}}_{t}={{\rho_w}}\, {{\varepsilon^w}}_{t-1}+{{\eta^{w}}}_{t}-{{\mu_w}}\, {{\sigma_{maw}}}\, {{\eta^{w}}}_{t-1}
\end{dmath}
% Equation 36
\begin{dmath}
{{\varepsilon^r}}_{t}={{\rho_r}}\, {{\varepsilon^r}}_{t-1}+{{\eta^m}}_{t}
\end{dmath}
% Equation 37
\begin{dmath}
{{\sigma_w}}_{t}={{\sigma_w}}_{t-1}\, {{\rho_{\sigma_w}}}+{{\eta^{\sigma_w}}}_{t}
\end{dmath}
% Equation 38
\begin{dmath}
{{\pi_*}}_{t}={{\rho_{\pi_*}}}\, {{\pi_*}}_{t-1}+{{\eta^{\pi_*}}}_{t}
\end{dmath}
% Equation 39
\begin{dmath}
{{z_p}}_{t}={{\rho_{zp}}}\, {{z_p}}_{t-1}+{{\eta^{z_p}}}_{t}
\end{dmath}
% Equation 40
\begin{dmath}
{{dlGDP}}_{t}={{w}}_{t}+{{y}}_{t}-{{y}}_{t-1}+{{\bar \gamma}}
\end{dmath}
% Equation 41
\begin{dmath}
{{dlCONS}}_{t}={{w}}_{t}+{{\bar \gamma}}+{{c}}_{t}-{{c}}_{t-1}
\end{dmath}
% Equation 42
\begin{dmath}
{{dlINV}}_{t}={{w}}_{t}+{{\bar \gamma}}+{{i}}_{t}-{{i}}_{t-1}
\end{dmath}
% Equation 43
\begin{dmath}
{{dlWAG}}_{t}={{w}}_{t}+{{\bar \gamma}}+{{w}}_{t}-{{w}}_{t-1}
\end{dmath}
% Equation 44
\begin{dmath}
{{lHOURS}}_{t}={{l}}_{t}+{{\bar l}}
\end{dmath}
% Equation 45
\begin{dmath}
{{FEDFUNDS}}_{t}={{r}}_{t}+{{\bar r}}
\end{dmath}
% Equation 46
\begin{dmath}
{{dlP}}_{t}={{\bar \pi}}+{{\pi}}_{t}
\end{dmath}
% Equation 47
\begin{dmath}
{{Spread}}_{t}=100\, \left({{r^{ktil}}}_{t}-{{r}}_{t}\right)+0.02
\end{dmath}
