\section{A more General Model}
Assuming not full depreciation $0 < \delta < 1$. The household's problem is
\[ 
U = E_t \sum_{t=0}^{\infty} \beta^i U(C_{t+i} , 1 - L_{t+i} )
\]
where the utility function is:
\[
U(C_t, 1-L_t) = \ln C_t + \theta \frac{(1-L_t)^{1-\gamma_l}}{1-\gamma_l}
\]
log in consumption, CES is leisure. $\gamma_l = 1$ shows log in leisure as well. 

\subsection{The log-linearized version}
Small letters denote the log-deviations from the non-stochastic BGP:
$c_t = \ln C_t - \ln C_t^{\ast}$, $l_t = \ln L_t - \ln L_t^{\ast}.$


\textcolor{blue}{1. The production function}
The production function is:
\[ Y_t = K_t^{\alpha} (A_t L_t)^{1-\alpha} \]
rewrite as:
\[ Y_t^{*} e^{y_t} = K^{*^{\alpha}} _t e^{\alpha k_t}(A_t^* L_t^*)^{1-\alpha }e^{(a_t + l_t)(1-\alpha )}  \]
and use the production function to get:
\[ y_t = \alpha k_t + (a_t + l_t)(1-\alpha ).\]

\textcolor{blue}{2. Capital accumulation}
$$K_{t+1}=(1-\delta)K_t+Y_t-C_t$$
re-write as
$$K_{t+1}^*e^{k_{t+1}}=(1-\delta)K_t^*e^{k_t}+Y_t^*e^{y_t}-C_t^*e^{c_t}$$
Now use the fact that for $x$ small enough $e^x\approx1+x$ to get:
$$K_{t+1}^{*}+K_{t+1}^{*}k_{t+1}\approx(1-\delta)K_{t}^{*}+(1-\delta)K_{t}^{*}k_{t}+Y_{t}^{*}+Y_{t}^{*}y_{t}-C_{t}^{*}-C_{t}^{*}c_{t}$$
which simplifies to
$$\frac{K_{t+1}^*}{K_t^*}k_{t+1}\approx(1-\delta)k_t+\frac{Y_t^*}{K_t^*}y_t-\frac{C_t^*}{K_t^*}c_t.$$

\textcolor{blue}{3. The rental rate}
$$R_t=\alpha\left(\frac{A_tL_t}{K_t}\right)^{1-\alpha}+(1-\delta)$$
rewrite as
$$R_t^*e^{r_t}=\alpha\left(\frac{A_t^*L^*}{K_t^*}\right)^{1-\alpha}e^{(1-\alpha)(a_t+l_t-k_t)}+(1-\delta)$$
this is approximately
$$R_t^*r_t\approx\alpha(1-\alpha)\left(\frac{A_t^*L^*}{K_t^*}\right)^{1-\alpha}(a_t+I_t-k_t).$$

\textcolor{blue}{4. The wage rate}
$$W_t=(1-\alpha)A_t^{1-\alpha}\left(\frac{K_t}{L_t}\right)^\alpha $$
re-write as
$$W_t^*e^{w_t}=(1-\alpha)A_t^{*^{1-\alpha}}e^{(1-\alpha)a_t}\left(\frac{K_t^*}{L_t^*}\right)^\alpha e^{\alpha(k_t-I_t)}$$
which simplifies to
$$w_t=(1-\alpha)a_t+\alpha(k_t-I_t).$$

\textcolor{blue}{5. The intra-temporal FOC}
$$\frac{W_t}{C_t}=\theta(1-L_t)^{-\gamma_l}$$
re-write and approximate:
$$\frac{W_t^*e^{W_t}}{C_t^*e^{C_t}}=\theta(1-L^*e^{I_t})^{-\gamma_l}\Rightarrow\frac{W_t^*+W_t^*w_t}{C_t^*+C_t^*c_t}\approx\theta(1-L^*-L^*I_t)^{-\gamma_l}$$
we do a first order taylor approximation around $c_t=w_t=I_t=0$:
$$\frac{W_t^*}{C_t^*}+\frac{W_t^*}{C_t^*}w_t-\frac{W_t^*}{C_t^*}c_t\approx\theta(1-L^*)^{-\gamma_l}+\theta\gamma_l(1-L^*)^{-\gamma_l-1}L^*I_t\\\frac{W_t^*}{C_t^*}(w_t-c_t)\approx\theta\gamma_l(1-L^*)^{-\gamma_l-1}L^*I_t$$
which simplifies to
$$w_t-c_t\approx\gamma_l\frac{L^*}{1-L^*}I_t.$$

\textcolor{blue}{6. The inter-temporal FOC}
$${C_t}=\beta E_t\left(\frac{R_{t+1}}{C_{t+1}}\right) $$
re-write as
$$C_t^*e^{C_t}=\beta E_t\left(\frac{R^*e^{r_{t+1}}}{C_{t+1}^*e^{c_{t+1}}}\right)$$
which is
$$e^{c_t}=E_t\left(\frac{e^{r_{t+1}}}{e^{c_{t+1}}}\right)\Rightarrow\frac1{1+c_t}\approx E_t\left(\frac{1+r_{t+1}}{1+c_{t+1}}\right)$$
finally, do a first order Taylor approximation
$$-c_t\approx E_t(r_{t+1}-c_{t+1}). $$

Blanchard-Kahn conditions
